

1. Comprobamos que  $A = LU$ .

$$A = \overbrace{\begin{pmatrix} 2 & 0 & 0 \\ -1 & 2 & 0 \\ 1 & -1 & 1 \end{pmatrix}}^L \cdot \overbrace{\begin{pmatrix} 4 & -3 & 1 \\ 0 & 4 & -3 \\ 0 & 0 & 2 \end{pmatrix}}^U = \begin{pmatrix} 8 & -6 & 2 \\ -4 & 11 & -3 \\ 4 & -7 & 6 \end{pmatrix} = A \quad \checkmark$$

Coincide.

2. Resolvemos  $Ax = b$ , utilizando  $A = LU$ .

$$Ax = b \rightarrow LUx = b$$

$\swarrow$   
 $Ly = b$

$\searrow$   
 $Ux = y$

Resolvemos el sistema  $Ly = b$ .

$$\begin{pmatrix} 2 & 0 & 0 \\ -1 & 2 & 0 \\ 1 & -1 & 1 \end{pmatrix} \cdot \begin{pmatrix} y_1 \\ y_2 \\ y_3 \end{pmatrix} = \begin{pmatrix} 28 \\ -40 \\ 33 \end{pmatrix} \Rightarrow \begin{cases} 2y_1 & = 28 \\ -y_1 + 2y_2 & = -40 \\ y_1 - y_2 + y_3 & = 33 \end{cases}$$

$$2y_1 = 28 \rightarrow y_1 = 14$$

$$-14 + 2y_2 = -40 \rightarrow y_2 = -\frac{26}{2} = -13$$

$$14 + 13 + y_3 = 33 \rightarrow y_3 = 6$$

Forward substitution

$$y = \begin{bmatrix} 14 \\ -13 \\ 6 \end{bmatrix}$$

Resolvemos el sistema  $Ux = y$

$$\begin{pmatrix} 4 & -3 & 1 \\ 0 & 4 & -3 \\ 0 & 0 & 2 \end{pmatrix} \cdot \begin{pmatrix} x_1 \\ x_2 \\ x_3 \end{pmatrix} = \begin{pmatrix} 14 \\ -13 \\ 6 \end{pmatrix} \Rightarrow \begin{cases} 4x_1 - 3x_2 + x_3 = 14 \\ 4x_2 - 3x_3 = -13 \\ 2x_3 = 6 \end{cases}$$

$$4x_1 + 3 + 3 = 14 \rightarrow x_1 = \frac{8}{4} = 2$$

$$4x_2 - 9 = -13 \rightarrow x_2 = -1$$

$$2x_3 = 6 \rightarrow x_3 = 3$$

Backward

substitution  $\Rightarrow$

$$\begin{bmatrix} 2 \\ -1 \\ 3 \end{bmatrix}$$